remove admits

examples/quantum/IBE_GPV.ec
@@ -131,20 +131,65 @@ proof. smt(ge0_cqh ge0_gqh). qed.
 op q = qe + qh + 1.
 
 (* --------------------------------------------------------------------------- *)
+import DBB Bool.
+
+(* FIXME: move this *)
+lemma dbfun_ll lam : is_lossless (dbfun lam).
+proof. apply/dfun_ll => /=; apply/Biased.dbiased_ll. qed.
+hint solve 0 random : dbfun_ll.
+
+module B (A:AdvIDCPA_QROM) : AdvCPA = {
+  import var IDCPA
+
+  var he : identity -> skey
+  var bf : identity -> bool
+
+  module E0 = {
+    proc extract(id:identity) : skey = {
+      log <- id::log;
+      return he id;
+    }
+  }
+
+  proc choose (lam_:real, k: mpkey * pkey) : msg * msg = {
+    var m1, m2, mpk, pk;
+    (mpk, pk) <- k;
+    log <- [];
+    bf <$ dbfun lam_;
+    he <$ dfskey;
+    QRO.h <- (fun m => if bf m then pk else f mpk (he m)); 
+    (id,m1,m2) <@ A(QRO,E0).choose(mpk);
+    return (m1,m2);
+  }
+
+  proc guess(c:cipher) : bool = {
+    var b';
+    b' <@ A(QRO,E0).guess(c);
+    if (!(bf id /\ (forall x', x' \in log => !bf x'))) b' <$ {0,1};
+    return b';
+  }
+    
+}.
 
 section.
 
-declare module E: EncScheme0 {-IDCPA, -QRO}.
+declare module E: EncScheme0 {-IDCPA, -QRO, -B}.
 
 declare module A : 
-  AdvIDCPA_QROM { -IDCPA, -QRO, -E }[choose : `{Inf, #H.h : cqh, #O.extract : cqe},
+  AdvIDCPA_QROM { -IDCPA, -QRO, -E, -B}[choose : `{Inf, #H.h : cqh, #O.extract : cqe},
                                  guess  : `{Inf, #H.h : gqh, #O.extract : gqe}].
 
 axiom A_wf : hoare [ IDCPA_QROM(A,GPV(E)).main : true ==> !IDCPA.id \in IDCPA.log /\
                                                           uniq IDCPA.log /\
                                                           size IDCPA.log = qe].
-(* FIXME: share this with FDH *)
-import DBB.
+
+axiom choose_ll (H <: QRO{-A}) (O <: OrclIBE{-A}) :
+   islossless O.extract => islossless H.h => islossless A(H, O).choose.
+
+axiom guess_ll (H <: QRO{-A}) (O <: OrclIBE{-A}) :
+  islossless O.extract => islossless H.h => islossless A(H, O).guess.
+
+axiom enc_ll : islossless E.enc.
 
 module type Init = {
   proc * init (h: identity -> pkey, lam_: real) : (identity -> bool) * (identity -> pkey)
@@ -172,12 +217,13 @@ local module G(I:Init) = {
 }.
 
 local lemma pr_split lam (I<:Init{-A,-E, -QRO}) &m :
+  islossless I.init =>
   equiv [I.init ~ I.init : ={arg} ==> ={res}] =>
   Pr[G(I).main(lam) @ &m : res] = 
    0.5 * (1.0 - Pr[G(I).main0(lam) @ &m : G.bf IDCPA.id /\ forall id', id' \in IDCPA.log => !G.bf id']) +
    Pr[G(I).main0(lam) @ &m : res /\ (G.bf IDCPA.id /\ forall id', id' \in IDCPA.log => !G.bf id')].
 proof.
-  move=> hI.
+  move=> I_ll hI.
   have -> : Pr[G(I).main(lam) @ &m : res] =
     Pr[G(I).main(lam) @ &m : 
       res /\ !(G.bf IDCPA.id /\ (forall id', id' \in IDCPA.log => !G.bf id')) \/
@@ -194,7 +240,10 @@ proof.
             true => //.
     + by conseq (: false) => /> //.
     + phoare split ! 1.0 r.
-      + admit. (* Need loosless adv *)
+      + islossless. 
+        + by apply (guess_ll QRO (<:IDCPA(A(QRO), GPV(E, QRO)).E)); islossless. 
+        + by apply enc_ll.              
+        by apply (choose_ll QRO (<:IDCPA(A(QRO), GPV(E, QRO)).E)); islossless. 
       call (: (glob A, glob E) = (glob A, glob E){m} /\ lam_ = lam ==> 
                G.bf IDCPA.id /\ forall (id' : identity), id' \in IDCPA.log => ! G.bf id'); 2: by auto.
       by bypr => &m0 h; rewrite /r; byequiv => //; sim; move: h => />.  
@@ -276,7 +325,10 @@ seq 1 : true 1.0 (lam*(1.0-lam)^qe)
         _ 0.0 
        (!IDCPA.id \in IDCPA.log /\ uniq IDCPA.log /\ size IDCPA.log = qe /\ lam_ = lam).
 + by call A_wf; auto.
-+ admit. (* Adversary lossless *)
++ islossless.
+  + by apply (guess_ll QRO (<:IDCPA(A(QRO), GPV(E, QRO)).E)); islossless.
+  + by apply enc_ll.
+  by apply (choose_ll QRO (<:IDCPA(A(QRO), GPV(E, QRO)).E)); islossless. 
 + rnd (fun t => t IDCPA.id /\ forall id', id' \in IDCPA.log => ! t id').
   skip => /> &1 hid hu hs.
   have /=:= dbfunE_mem_uniq lam [IDCPA.id{1}] IDCPA.log{1} lam_bound _ hu _.
@@ -307,7 +359,8 @@ proof.
   have ->:  
    Pr[G(Init1).main(lam) @ &m : res] - 0.5 =
      (lam * (1.0-lam)^qe) * (Pr[IDCPA_QROM(A,GPV(E)).main() @ &m : res] - 0.5).
-  + rewrite (pr_split lam Init1); 1: by sim.
+  + rewrite (pr_split lam Init1); 2: by sim.
+    + islossless => *. 
     by rewrite pr_GI1 1:// pr_GI1t 1://; ring.
   by have := mul_le_pow lam qe hlam' ge0_qe; smt(mu_bounded).
 qed.
@@ -357,7 +410,10 @@ local lemma l2 &m lam :
    (2%r * q%r + qe%r + 1%r) / 4.0 * lam ^2.
 proof.
   move=> lam_bound.
-  rewrite (pr_split lam Init2); 1: (by sim); rewrite (pr_split lam Init1); 1: by sim.
+  rewrite (pr_split lam Init2).
+  + by islossless. + by sim.
+  rewrite (pr_split lam Init1).
+  + by islossless. + by sim.
   rewrite (pr_size (fun _ => true) Init1) (pr_size (fun _ => true) Init2).
   rewrite (pr_size idfun Init1) (pr_size idfun Init2) /idfun /=.
   apply (ler_trans 
@@ -387,43 +443,142 @@ proof.
   + admit.
 qed.
 
-module B (A:AdvIDCPA_QROM) : AdvCPA = {
-  import var IDCPA
-
-  var he : identity -> skey
-  var bf : identity -> bool
-
-  module E0 = {
-    proc extract(id:identity) : skey = {
-      log <- id::log;
-      return he id;
-    }
+import Bool.
+local module S = {
+  proc sample1 () = {
+    var r;
+    r <$ dpkey; 
+    return r;
   }
-
-  proc choose (lam_:real, k: mpkey * pkey) : msg * msg = {
-    var m1, m2, mpk, pk;
-    (mpk, pk) <- k;
-    log <- [];
-    bf <$ dbfun lam_;
-    he <$ dfskey;
-    QRO.h <- (fun m => if bf m then pk else f mpk (he m)); 
-    (id,m1,m2) <@ A(QRO,E0).choose(mpk);
-    return (m1,m2);
+  proc sample2 (mpk:mpkey, msk:mskey) = {
+    var z;
+    z <$ sampleD;
+    return f mpk z;
   }
+}.
 
-  proc guess(c:cipher) : bool = {
-    var b';
-    b' <@ A(QRO,E0).guess(c);
-    if (!(bf id /\ (forall x', x' \in log => !bf x'))) b' <$ {0,1};
-    return b';
-  }
-    
+module type OrclPK  = {
+  proc pkey(id:identity) : pkey
+}.
+
+quantum module type AdvIDCPA_QROM_aux (H : QRO, O : OrclIBE, P:OrclPK)  = {
+  proc choose (mpk : mpkey): identity * msg * msg 
+  
+  proc guess (c : cipher): bool
 }.
 
 local lemma l3 &m lam : 
    Pr[G(Init2).main(lam) @ &m : res] = Pr[CPA(B(A), ES(E)).main(lam) @ &m : res].
 proof.
-admitted.
+byequiv => //; proc.
+inline *.
+seq 11 10 : 
+  ((forall id', B.bf id' => pk = (mpk0, QRO.h id')){2} /\
+   (forall id', !G.bf{1} id' => QRO.h{1} id' = f IDCPA.mpk{1} (B.he{2} id')) /\
+   ={QRO.h, IDCPA.log, glob A, glob E} /\ G.bf{1} = B.bf{2} /\ IDCPA.mpk{1} = mpk0{2} /\ 
+   (IDCPA.mpk,IDCPA.msk){1} \in kg).
++ conseq />.
+  swap{1} 10 -9; swap{1} [3..4] 3; swap{1} [2..3] 1; wp.
+  rnd (fun (h: identity -> pkey) => fun id => finv msk{2} (h id))
+      (fun (h: identity -> skey) => fun id => f mpk{2} (h id)).
+  rnd; wp.
+  seq 1 1: (i{2} = lam_{1} /\ keys{1} = (mpk, msk){2} /\ keys{1} \in kg).
+  + auto => /> /#. 
+    conseq (: i{2} = lam_{1} /\ keys{1} = (mpk{2}, msk{2}) /\ (keys{1} \in kg) /\
+              y{1} = f mpk{2} sk0{2}).
+    + move=> /> &1 &2 hin sk bf hbf; split.
+      + by move=> he _; apply fun_ext => z; rewrite (finv_f _ _ hin).
+      move=> _; split.
+      + move=> *; apply dfskey_dfpkey.
+      move=> _ h _; split.
+      + by apply fun_ext => z; rewrite (f_finv _ _ hin).
+      move=> _; split.
+      + by move=> z _; rewrite (f_finv _ _ hin).
+      by apply fun_ext => z; rewrite (f_finv _ _ hin).
+   conseq (: keys{1} \in kg /\ keys{1} = (mpk, msk){2} ==> y{1} = f mpk{2} sk0{2}) => //.
+   transitivity{1} {y <@ S.sample1(); }
+     (true ==> ={y})
+     (keys{1} \in kg /\ keys{1} = (mpk, msk){2} ==> y{1} = f mpk{2} sk0{2}) => //.
+   + smt().
+   + by inline *;auto.
+   transitivity{1}{y <@ S.sample2(keys);}
+     (keys{2} \in kg ==> ={y})
+     (keys{1} = (mpk{2}, msk{2}) ==> y{1} = f mpk{2} sk0{2}) => //; last by inline *; auto.
+   + smt().
+   call (: arg{2} \in kg ==> ={res}) => //.
+   bypr (res{1}) (res{2}) => //.
+   move=> &1 &2 a harg. 
+   have -> : Pr[S.sample1() @ &1 : res = a] = mu1 dpkey a.
+   + by byphoare => //; proc; rnd; skip.
+   have -> : Pr[S.sample2(mpk{2}, msk{2}) @ &2 : res = a] = mu1 (dmap sampleD (f mpk{2})) a.
+   + by byphoare (_: arg = (mpk,msk){2} ==> res = a) => //; proc; rnd; skip => />; rewrite dmap1E.
+   by admit. (* both distribution are funiform *)
+
+seq 10 6 : ( (!G.bf IDCPA.id \/ exists m', m' \in IDCPA.log /\ G.bf m'){1} = 
+              (!B.bf IDCPA.id \/ exists m', m' \in IDCPA.log /\ B.bf m'){2} /\
+            (!(!G.bf IDCPA.id \/ exists m', m' \in IDCPA.log /\ G.bf m'){1} => 
+             ={IDCPA.id,m1 ,m2} /\ (IDCPA.b, IDCPA.b', G.bf){1} = (b, b'0,B.bf){2})); last first.
++ wp; sp; if{1}.
+  + by rcondf{2} 1 => *; auto => /> /#.
+  rcondt{2} 1 => *; 1: by auto => /> /#.
+  by rnd (fun b1 => !(b{2} ^^ b1)); skip => /> /#.
+
+seq 1 2 : 
+  ( (forall (id' : identity), B.bf{2} id' => pk{2} = (mpk0{2}, QRO.h{2} id')) /\
+    (forall (id' : identity), ! G.bf{1} id' => QRO.h{1} id' = f IDCPA.mpk{1} (B.he{2} id')) /\
+     ={QRO.h} /\  G.bf{1} = B.bf{2} /\ IDCPA.mpk{1} = mpk0{2} /\ (IDCPA.mpk{1}, IDCPA.msk{1}) \in kg /\
+    (exists m', m' \in IDCPA.log /\ G.bf m'){1} = (exists m', m' \in IDCPA.log /\ B.bf m'){2} /\
+    (!(exists m', m' \in IDCPA.log /\ G.bf m'){1} => 
+        ={IDCPA.id,m1 ,m2, glob A, glob E, IDCPA.log} /\ G.bf{1} = B.bf{2})).
++ wp.
+  call (: (exists m', m' \in IDCPA.log /\ B.bf m'), 
+          (={IDCPA.log, QRO.h} /\ G.bf{1} = B.bf{2} /\
+           (forall id', !G.bf{1} id' => QRO.h{1} id' = f IDCPA.mpk{1} (B.he{2} id')) /\
+          (IDCPA.mpk,IDCPA.msk){1} \in kg),
+          (exists m', m' \in IDCPA.log /\ G.bf m'){1} =
+          (exists m', m' \in IDCPA.log /\ B.bf m'){2}
+          ).
+  + by apply choose_ll.
+  + by proc; inline *; wp; skip => />; smt(finv_f).
+  + by move=> &2 ?; proc; inline *; auto; smt().
+  + by move=> &1; proc; inline *; auto; smt().
+  + by proc; skip => />.
+  + by move=> *;proc; skip => />.
+  + by move=> *;proc; skip => />.
+  by skip => /> /#.
+wp; case: ((!G.bf IDCPA.id \/ exists (m' : identity), (m' \in IDCPA.log) /\ G.bf m'){1}).
++ call{1} (: (!G.bf IDCPA.id \/ exists (m' : identity), (m' \in IDCPA.log) /\ G.bf m') ==> 
+             (!G.bf IDCPA.id \/ exists (m' : identity), (m' \in IDCPA.log) /\ G.bf m')).
+  conseq (:true ==> true) (: _ ==> _) => //.
+  + proc (!G.bf IDCPA.id \/ exists (m' : identity), (m' \in IDCPA.log) /\ G.bf m') => //. 
+    + by proc; inline *; auto; smt().
+    by move=> *;proc; skip => />.
+  by apply (guess_ll QRO (<:IDCPA(A(QRO), GPV(E, QRO)).E));islossless.
++ call{2} (: (!B.bf IDCPA.id \/ exists (m' : identity), (m' \in IDCPA.log) /\ B.bf m') ==> 
+             (!B.bf IDCPA.id \/ exists (m' : identity), (m' \in IDCPA.log) /\ B.bf m')).
+  + conseq (:true ==> true) (: _ ==> _) => //.
+    + proc (!B.bf IDCPA.id \/ exists (m' : identity), (m' \in IDCPA.log) /\ B.bf m') => //. 
+      + by proc; inline *; auto; smt().
+      by move=> *;proc; skip => />.
+    by apply (guess_ll QRO (<:B(A).E0)); islossless.
+  wp;call{1} enc_ll; call{2} enc_ll.
+  by wp; rnd; skip => /> /#.
+call (: (exists m', m' \in IDCPA.log /\ B.bf m'), 
+        (={IDCPA.log, QRO.h} /\ G.bf{1} = B.bf{2} /\
+         (forall id', !G.bf{1} id' => QRO.h{1} id' = f IDCPA.mpk{1} (B.he{2} id')) /\
+        (IDCPA.mpk,IDCPA.msk){1} \in kg),
+        (exists m', m' \in IDCPA.log /\ G.bf m'){1} =
+        (exists m', m' \in IDCPA.log /\ B.bf m'){2}
+        ).
++ by apply guess_ll.
++ by proc; inline *; wp; skip => />; smt(finv_f).
++ by move=> &2 ?; proc; inline *; auto; smt().
++ by move=> &1; proc; inline *; auto; smt().
++ by proc; skip => />.
++ by move=> *;proc; skip => />.
++ by move=> *;proc; skip => />.
+wp; call(:true); wp; rnd; skip => /#.
+qed.
 
 local lemma l4 &m lam: 
   0.0 < lam <= 1.0 =>
@@ -434,17 +589,18 @@ proof. move: (l1 &m) (l2 &m) (l3 &m) => /#. qed.
 
 local lemma conclusion &m:
   let eps = `|Pr[IDCPA_QROM(A,GPV(E)).main() @ &m : res] - 0.5| in
-  let lam = 2.0 * eps / (2%r * q%r + 5.0*qe%r + 1%r) in 
+  let lam = (2.0 * eps) / (2%r * q%r + 5.0*qe%r + 1%r) in 
   eps^2 / (2%r * q%r + 5.0*qe%r + 1%r) <=
      `|Pr[CPA(B(A), ES(E)).main(lam) @ &m : res]- 0.5|.
 proof.
   move=> eps; case: (eps = 0%r).
   + by move: eps => />; rewrite expr2 /= /#.
   move=> heps lam.
+  have h1 : 0%r < (2%r * q%r + 5%r * qe%r + 1%r) by smt(ge0_qh ge0_qe).
   have := l4 &m lam _.
-  + admit.
+  + rewrite ler_pdivr_mulr => //; smt(mu_bounded). 
   apply/ler_trans/lerr_eq; rewrite -/eps /lam;field => //.
-  admit.
+  smt(). 
 qed.
 
 end section.
